src/Spec/Proc.v
@@ -9,26 +9,52 @@ Set Warnings "-undeclared-scope".
 
 Import RelationNotations.
 
-(** Syntax: free monad over a type family of operations *)
-Inductive proc (Op: Type -> Type) (T : Type) : Type :=
-| Call (op : Op T)
-| Ret (v : T)
-| Bind (T1 : Type) (p1 : proc Op T1) (p2 : T1 -> proc Op T).
+Section Proc.
+  Variable Op : Type -> Type.
+
+  Inductive proc : Type -> Type :=
+  | Call : forall T (op : Op T), proc T
+  | Ret : forall T (v : T), proc T
+  | Bind : forall T (T1 : Type) (p1 : proc T1) (p2 : T1 -> proc T), proc T
+  (* TODO: why is p's argument an option in until? *)
+  | Until : forall T (c : T -> bool) (p : option T -> proc T) (v : option T), proc T
+  | Spawn : forall T (p: proc T), proc unit.
+
+End Proc.
+
 Arguments Call {Op T}.
 Arguments Ret {Op T} v.
+Arguments Until {Op T} _ _ _.
+Arguments Spawn {Op} _.
 
-(** A sequence of procedures that a user might wish to run, where for each
-    procedure in the sequence they specify a continuation to run on success,
-    and an alternate sequence to run if a crash happens. *)
+(*
 Inductive proc_seq (Op: Type -> Type) (R: Type) : Type :=
 | Seq_Nil
 | Seq_Bind (T : Type) (p : proc Op T) (rx : T + R -> proc_seq Op R).
 Arguments Seq_Nil {Op R}.
 Arguments Seq_Bind {Op R T}.
+*)
 
-(** Semantics: defined using big-step execution relations *)
+(* TODO : allow forwarding the recovery value to the next routine *)
+Inductive rec_seq (Op: Type -> Type) : Type :=
+| Seq_Nil
+| Seq_Cons (T : Type) (p : proc Op T) (ps: rec_seq Op).
+Arguments Seq_Nil {Op}.
+Arguments Seq_Cons {Op T}.
 
-Definition OpSemantics Op State := forall T, Op T -> relation State State T.
+Fixpoint rec_seq_append Op (ps1 ps2: rec_seq Op) :=
+  match ps1 with
+  | Seq_Nil => ps2
+  | Seq_Cons p ps1' => Seq_Cons p (rec_seq_append ps1' ps2)
+  end.
+
+Definition rec_seq_snoc Op T (ps: rec_seq Op) (p: proc Op T) :=
+  rec_seq_append ps (Seq_Cons p Seq_Nil).
+
+Definition thread_pool (Op: Type -> Type) := list {T : Type & proc Op T}.
+
+Definition OpSemantics Op State :=
+  forall T, Op T -> relation State State T.
 Definition CrashSemantics State := relation State State unit.
 
 Record Dynamics Op State :=
@@ -38,54 +64,115 @@ Record Dynamics Op State :=
 Section Dynamics.
 
   Context `(sem: Dynamics Op State).
-  Notation proc := (proc Op).
-  Notation proc_seq := (proc_seq Op).
-  Notation step := sem.(step).
-  Notation crash_step := sem.(crash_step).
 
   (** First, we define semantics of running programs with halting (without the
   effect of a crash or recovery) *)
 
-  Fixpoint exec {T} (p: proc T) : relation State State T :=
+  Definition until1 T (c : T -> bool)
+                      (p : option T -> proc Op T)
+                      (v : option T) :=
+    Bind (p v) (fun x => if c x then Ret x else Until c p (Some x)).
+   
+  Fixpoint exec_step {T} (p: proc Op T)
+    : relation State State (proc Op T * thread_pool Op) :=
     match p with
-    | Ret v => pure v
-    | Call op => step op
-    | Bind p p' => v <- exec p; exec (p' v)
+    | Ret v => pure (Ret v, nil)
+    | Call op => v <- step sem op; pure (Ret v, nil)
+    | @Bind _ T0 _ p p' =>
+      vp <- exec_step p;
+      (let (p1, t) := vp in
+       match p1 in (proc _ T1) return
+             (T1 -> proc _ T0) -> relation State State (proc _ T0 * thread_pool _)
+       with
+        | Ret v => fun p' => pure (p' v, t)
+        | p => fun p' => pure (Bind p p',t)
+        end) p'
+    | Until c p v  => pure (until1 c p v, nil)
+    | Spawn T' p' => pure (Ret tt, existT _ T' p' :: nil)
     end.
 
-  Fixpoint exec_halt {T} (p: proc T) : relation State State unit :=
-    match p with
-    | Ret v => pure tt
-    | Call op => pure tt + (step op;; pure tt)
-    | Bind p p' =>
-      (* note that this pure tt case is redundant (since the base cases already
-      include it) but is included for a more obvious definition *)
-      pure tt +
-      exec_halt p +
-      (v <- exec p;
-         exec_halt (p' v))
+  (* TODO: need to define this after, otherwise can't use proc in the above *)
+  Notation proc := (proc Op).
+  Notation rec_seq := (rec_seq Op).
+  Notation thread_pool := (thread_pool Op).
+  Notation step := sem.(step).
+  Notation crash_step := sem.(crash_step).
+
+  Definition exec_pool_hd {T} (p: proc T) (ps: thread_pool)
+    : relation State State thread_pool :=
+    pps <- exec_step p;
+    pure (existT _ T (fst pps) :: ps ++ snd pps).
+
+  Fixpoint exec_pool (ps: list {T & proc T})
+    : relation State State thread_pool :=
+    match ps with
+    | nil => pure nil
+    | existT _ T p :: nil => exec_pool_hd p nil
+    | existT _ T p :: ps' =>
+      (exec_pool_hd p ps') +
+      (ps'_upd <- exec_pool ps';
+       pure (existT _ T p :: ps'_upd))
     end.
 
-  Definition exec_recover {R} (rec: proc R) : relation State State R :=
-    seq_star (exec_halt rec;; crash_step);;
-             exec rec.
+  Definition exec_partial {T} (p: proc T) :=
+    bind_star (exec_pool) ((existT _ T p) :: nil).
 
-  Definition exec_recover_unfold {R} (rec: proc R) :
+  Definition exec_halt {T} (p: proc T) : relation State State unit :=
+    exec_partial p;; pure tt.
+
+  (* A complete execution is one in which the first thread is a value *)
+  Definition exec {T} (p: proc T) : relation State State {T: Type & T} :=
+    ps <- exec_partial p;
+    match ps with
+    | existT _ _ (Ret v) :: _ => pure (existT _ _ v)
+    | _ => @none _ _ {T: Type & T}
+    end.
+
+  Fixpoint exec_seq_partial (ps: rec_seq) : relation State State unit :=
+    match ps with
+    | Seq_Nil => pure tt
+    | Seq_Cons p ps => (exec p;; exec_seq_partial ps) + (exec_partial p;; pure tt)
+    end.
+
+  Fixpoint exec_seq (ps: rec_seq) : relation State State unit :=
+    match ps with
+    | Seq_Nil => pure tt
+    | Seq_Cons p ps => exec p;; exec_seq ps
+    end.
+
+  Definition exec_recover1 T (rec: proc T) : relation State State unit :=
+    seq_star (exec_partial rec;; crash_step);;
+             exec rec;; pure tt.
+
+  Definition exec_recover (rec: rec_seq) : relation State State unit :=
+    seq_star (exec_seq_partial rec;; crash_step);;
+             exec_seq rec.
+
+  Definition exec_recover_unfold (rec: rec_seq) :
     exec_recover rec =
-    seq_star (exec_halt rec;; crash_step);;
-             exec rec := eq_refl.
+    seq_star (exec_seq_partial rec;; crash_step);;
+             exec_seq rec := eq_refl.
 
   (* recovery execution *)
-  Definition rexec {T R} (p: proc T) (rec: proc R) : relation State State R :=
-      exec_halt p;; crash_step;; exec_recover rec.
+  Definition rexec {T} (p: proc T) (rec: rec_seq) :=
+      exec_partial p;; crash_step;; exec_recover rec.
 
-  Definition rexec_unfold {T R} (p: proc T) (rec: proc R) :
+  Definition rexec_unfold {T} (p: proc T) (rec: rec_seq) :
     rexec p rec =
-    exec_halt p;; crash_step;; exec_recover rec := eq_refl.
+    exec_partial p;; crash_step;; exec_recover rec := eq_refl.
 
-  Definition exec_or_rexec {T R} (p : proc T) (rec: proc R) : relation State State (T + R) :=
+  Definition rexec_seq (ps: rec_seq) (rec: rec_seq) :=
+      exec_seq_partial ps;; crash_step;; exec_recover rec.
+
+  Definition rexec_seq_unfold (ps: rec_seq) (rec: rec_seq) :
+    rexec_seq ps rec =
+    exec_seq_partial ps;; crash_step;; exec_recover rec := eq_refl.
+
+  Definition exec_or_rexec {T} (p : proc T) (rec: rec_seq) :=
     (v <- exec p; pure (inl v)) + (v <- rexec p rec; pure (inr v)).
 
+  (* TODO: need to track that the hd type does not change for this to make sense *)
+  (*
   Fixpoint exec_seq {R} (p: proc_seq R) (rec: proc R)
     : relation State State (list {X : Type & X}) :=
     match p with
@@ -106,6 +193,7 @@ Section Dynamics.
       pure (existT _ _ v :: l)
     end.
   Proof. destruct p; auto. Qed.
+   *)
 
 End Dynamics.
 
