src/Helpers/RelationRewriting.v
@@ -44,6 +44,10 @@ Ltac setoid_norm_goal :=
     setoid_rewrite unit_identity
   | |- context[rel_or _ (rel_or _ _)] =>
     setoid_rewrite rel_or_assoc
+  | |- context[and_then (none) _] =>
+    setoid_rewrite none_absorb_l
+  | |- context[and_then _ (fun _ => none)] =>
+    setoid_rewrite none_absorb_r
   end.
 
 Ltac setoid_norm_hyp H :=
