src/Spec/ProcTheorems.v
@@ -11,38 +11,59 @@ Import RelationNotations.
 Section Dynamics.
   Context `(sem: Dynamics Op State).
   Notation proc := (proc Op).
+  Notation rec_seq := (rec_seq Op).
   Notation step := sem.(step).
   Notation crash_step := sem.(crash_step).
   Notation exec_halt := sem.(exec_halt).
+  Notation exec_partial := sem.(exec_partial).
   Notation exec := sem.(exec).
+  Notation exec_seq_partial := sem.(exec_seq_partial).
+  Notation exec_seq := sem.(exec_seq).
+  Notation rexec_seq := sem.(rexec_seq).
+  Notation exec_recover1 := sem.(exec_recover1).
   Notation exec_recover := sem.(exec_recover).
   Notation rexec := sem.(rexec).
 
   Hint Resolve rimpl_refl requiv_refl.
 
+  Ltac destruct_hd :=
+    match goal with
+    | [ |- and_then (match ?v with | _ => _  end) _ ---> _ ] => destruct v
+    end.
+
   Theorem exec_halt_finish T (p: proc T) :
     exec p;; pure tt ---> exec_halt p.
   Proof.
-    induction p; simpl in *; norm.
-    - rewrite <- rel_or_intror.
-      reflexivity.
-    - setoid_rewrite H.
-      rewrite <- rel_or_intror.
-      eauto.
+    unfold exec, exec_halt; induction p; simpl in *; norm; try rel_congruence;
+      repeat destruct_hd; norm; apply from_none.
   Qed.
 
   Theorem exec_halt_noop T (p: proc T) :
     pure tt ---> exec_halt p.
   Proof.
-    induction p; simpl in *; norm.
-    - rewrite <- rel_or_introl; auto.
-    - rewrite <- rel_or_introl, <- rel_or_introl; auto.
+    unfold exec_halt. setoid_rewrite <-bind_star_expand_r. Left.
+  Qed.
+
+  Theorem exec_seq_partial_noop (p: rec_seq) :
+    pure tt ---> exec_seq_partial p.
+  Proof.
+    induction p; simpl; eauto.
+    Right. apply exec_halt_noop.
+  Qed.
+
+  Lemma exec_partial_ret T (v: T) :
+    exec_partial (Ret v) <---> pure (existT _ _ (Ret v) :: nil)%list.
+  Proof.
+    apply rimpl_to_requiv.
+    - unfold exec_partial. apply bind_star_ind_r_pure.
+      Split. simpl in *. unfold exec_pool_hd. simpl in *. norm.
+    - setoid_rewrite <-bind_star_expand_r. Left.
   Qed.
 
   Theorem exec_halt_ret T (v: T) :
     exec_halt (Ret v) <---> pure tt.
   Proof.
-    reflexivity.
+    unfold exec_halt. rew exec_partial_ret.
   Qed.
 
   Theorem exec_halt_idem T (p: proc T) :
@@ -51,9 +72,19 @@ Section Dynamics.
     apply rimpl_or; auto using exec_halt_noop.
   Qed.
 
+  Theorem exec_seq_partial_idem (p: rec_seq) :
+    pure tt + exec_seq_partial p <---> exec_seq_partial p.
+  Proof.
+    apply rimpl_or; auto using exec_seq_partial_noop.
+  Qed.
+
   Definition exec_equiv T (p p': proc T) :=
     exec p <---> exec p' /\
     exec_halt p <---> exec_halt p'.
+
+  Definition exec_seq_equiv (p p': rec_seq) :=
+    exec_seq p <---> exec_seq p' /\
+    exec_seq_partial p <---> exec_seq_partial p'.
 
   Global Instance exec_equiv_equiv T : Equivalence (exec_equiv (T:=T)).
   Proof.
@@ -72,57 +103,200 @@ Section Dynamics.
 
   Infix "<==>" := exec_equiv (at level 70).
 
-  Theorem rexec_equiv T (p p': proc T) R (rec: proc R) :
+  (* TODO: there is a more general theorem of this form *)
+  Lemma exec_partial_crash_pure T (p: proc T):
+    _ <- exec_partial p; crash_step <---> _ <- (exec_partial p;; pure tt); crash_step.
+  Proof. rewrite bind_assoc. norm. Qed.
+
+  Theorem rexec_equiv T (p p': proc T) (rec: rec_seq) :
     p <==> p' ->
     rexec p rec <---> rexec p' rec.
   Proof.
     unfold "<==>"; propositional.
-    unfold rexec.
-    rew H0.
+    unfold rexec. norm.
+    unfold exec_halt in H0.
+    setoid_rewrite <-bind_assoc.
+    rel_congruence.
+    rewrite exec_partial_crash_pure.
+    rewrite H0.
+    norm.
   Qed.
 
   Global Instance exec_respectful T:
-    Proper (@exec_equiv T ==> @requiv State State T) exec.
+    Proper (@exec_equiv T ==> @requiv State State _) exec.
   Proof. intros ?? (?&?); intuition. Qed.
 
   Global Instance exec_halt_respectful T:
     Proper (@exec_equiv T ==> @requiv State State unit) exec_halt.
   Proof. intros ?? (?&?); intuition. Qed.
 
-  Global Instance rexec_respectful T R:
-    Proper (@exec_equiv T ==> eq ==> @requiv State State R) rexec.
+  Global Instance rexec_respectful T:
+    Proper (@exec_equiv T ==> @eq (rec_seq) ==> @requiv State State _) rexec.
   Proof. intros ?? ? ?? ->. eapply rexec_equiv; eauto. Qed.
 
   Theorem monad_left_id T T' (p: T' -> proc T) v :
       Bind (Ret v) p <==> p v.
   Proof.
     split; simpl; norm.
-    rew rel_or_idem.
-    rew exec_halt_idem.
+    - unfold exec, exec_partial.
+      apply rimpl_to_requiv.
+      * rew<- bind_star_expand.
+        Split; [ apply from_none |]. 
+        simpl. unfold exec_pool_hd; norm; simpl.
+        setoid_rewrite <-bind_star_expand at 1.
+        rel_congruence; simpl. unfold exec_pool_hd; norm.
+      * setoid_rewrite <-bind_star_expand at 2.
+        Right. simpl. unfold exec_pool_hd; norm.
+    - unfold exec_halt, exec_partial.
+      apply rimpl_to_requiv.
+      * setoid_rewrite <-bind_star_expand at 1; norm.
+        Split; [rew<- bind_star_expand; Left|].
+        simpl. unfold exec_pool_hd; norm; simpl.
+      * setoid_rewrite <-bind_star_expand at 2; norm.
+        Right.
+        simpl. unfold exec_pool_hd; norm; simpl.
   Qed.
 
+  (*
   Theorem monad_assoc
           `(p1: proc T1)
           `(p2: T1 -> proc T2)
           `(p3: T2 -> proc T3) :
     Bind (Bind p1 p2) p3 <==> Bind p1 (fun v => Bind (p2 v) p3).
   Proof.
-    split; simpl; norm.
-    rew rel_or_idem.
-    rew exec_halt_idem.
-    repeat setoid_rewrite bind_dist_l.
+    induction p1.
+    - split; simpl; norm.
+      unfold exec. exec_partial.
+  Qed.
+   *)
+
+  Lemma exec_seq_partial_nil: exec_seq_partial Seq_Nil <---> pure tt.
+  Proof. eauto. Qed.
+  
+  Lemma exec_seq_nil: exec_seq Seq_Nil <---> pure tt.
+  Proof. eauto. Qed.
+
+  Lemma exec_recover_nil: exec_recover Seq_Nil <---> seq_star (crash_step).
+  Proof.
+    unfold exec_recover.
+    setoid_rewrite exec_seq_partial_nil.
+    norm. apply bind_right_id_unit.
+  Qed.
+
+  Opaque Proc.exec.
+
+
+  Lemma exec_seq_snoc T `(p: proc T) `(rec: rec_seq ):
+    exec_seq (rec_seq_snoc rec p) <--->
+             (exec_seq rec;; exec p;; pure tt).
+  Proof.
+    induction rec.
+    - simpl. norm.
+    - simpl. rew IHrec.
+  Qed.
+
+  Lemma exec_seq_append `(rec1: rec_seq) (rec2: rec_seq):
+    exec_seq (rec_seq_append rec1 rec2) <--->
+             (exec_seq rec1;; exec_seq rec2).
+  Proof.
+    induction rec1.
+    - simpl. norm.
+    - simpl. rew IHrec1.
+  Qed.
+
+  Lemma exec_seq_partial_snoc T `(p: proc T) `(rec: rec_seq ):
+    exec_seq_partial (rec_seq_snoc rec p) <--->
+                     (exec_seq_partial rec + (exec_seq rec ;; exec_halt p)).
+  Proof.
+    induction rec.
+    - simpl. rewrite bind_left_id, exec_halt_idem. apply rimpl_to_requiv.
+      * rewrite exec_halt_finish, rel_or_idem; auto.
+      * Right.
+    - simpl. setoid_rewrite IHrec.
+      rewrite bind_dist_l.
+      norm.
+      rewrite <-rel_or_assoc.
+      rewrite <-rel_or_assoc.
+      apply or_respects_equiv; eauto.
+      apply rel_or_symmetric.
+  Qed.
+
+  Lemma exec_seq_partial_append `(rec1: rec_seq) `(rec2: rec_seq):
+    exec_seq_partial (rec_seq_append rec1 rec2) <--->
+                     (exec_seq_partial rec1 + (exec_seq rec1 ;; exec_seq_partial rec2)).
+  Proof.
+    induction rec1.
+    - simpl. rewrite bind_left_id, exec_seq_partial_idem; auto.
+    - simpl. setoid_rewrite IHrec1.
+      rewrite bind_dist_l.
+      norm.
+      rewrite <-rel_or_assoc.
+      rewrite <-rel_or_assoc.
+      apply or_respects_equiv; eauto.
+      apply rel_or_symmetric.
+  Qed.
+
+  (* TODO: this is probably unneeded *)
+  Theorem exec_recover_snoc T `(p: proc T) `(rec: rec_seq) :
+    exec_recover (rec_seq_snoc rec p) <--->
+                 (exec_recover rec;;
+                  seq_star (rexec p rec);;
+                  exec p;; pure tt).
+  Proof.
+    unfold exec_recover.
+    unfold exec_recover, rexec, rexec_seq; simpl; norm.
+    rewrite exec_seq_partial_snoc.
+    rewrite ?bind_dist_r.
+    unfold exec_recover.
+    setoid_rewrite exec_seq_snoc.
+    gen (exec_seq rec) (exec_seq_partial rec) crash_step;
+      clear rec.
+    intros rec1 rec1_crash crash.
+    rew denesting.
+    rel_congruence.
+    rewrite <- ?bind_assoc.
+    rel_congruence; norm.
+    rewrite <-bind_assoc.
+    rewrite seq_unit_sliding_equiv.
     norm.
   Qed.
 
+  Theorem exec_recover_append
+          `(rec1: rec_seq)
+          `(rec2: rec_seq) :
+    exec_recover (rec_seq_append rec1 rec2) <--->
+                 (exec_recover rec1;;
+                  seq_star (rexec_seq rec2 rec1);;
+                  exec_seq (rec2)).
+  Proof.
+    unfold exec_recover.
+    unfold exec_recover, rexec, rexec_seq; simpl; norm.
+    rewrite exec_seq_partial_append.
+    rewrite ?bind_dist_r.
+    unfold exec_recover.
+    setoid_rewrite exec_seq_append.
+    gen (exec_seq rec1) (exec_seq_partial rec1) crash_step;
+      clear rec1.
+    intros rec1 rec1_crash crash.
+    rew denesting.
+    rel_congruence.
+    rewrite <- ?bind_assoc.
+    rel_congruence; norm.
+    rewrite seq_unit_sliding_equiv.
+    norm.
+  Qed.
+
+  (*
   Theorem exec_recover_bind
-          `(rec1: proc R)
-          `(rec2: R -> proc R') :
-    exec_recover (Bind rec1 rec2) <--->
+          `(rec1: proc unit)
+          `(rec2: proc unit) :
+    exec_recover (Bind rec1 (fun _ => rec2)) <--->
                  (v <- exec_recover rec1;
-                    v' <- bind_star (fun v => rexec (rec2 v) rec1) v;
-                    exec (rec2 v')).
+                    v' <- bind_star (fun v => rexec rec2 rec1) v;
+                    exec (rec2)).
   Proof.
     repeat unfold exec_recover, rexec; simpl; norm.
+    rew denesting.
 
     rewrite exec_halt_idem.
     rewrite ?bind_dist_r; norm.
@@ -138,9 +312,11 @@ Section Dynamics.
     rel_congruence; norm.
     rew bind_sliding.
   Qed.
+   *)
 
+  (*
   Theorem rexec_to_exec_recover
-          `(rec: proc R) :
+          `(rec: rec_seq) :
     rexec rec rec ---> exec_recover rec.
   Proof.
     unfold rexec, exec_recover.
@@ -149,26 +325,25 @@ Section Dynamics.
     rew seq_star1.
   Qed.
 
-  Theorem exec_recover_to_rexec
-          `(rec: proc R) :
-    crash_step;; exec_recover rec ---> rexec rec rec.
-  Proof.
-    unfold rexec, exec_recover.
-    setoid_rewrite <- exec_halt_noop at 2; norm.
-  Qed.
-
   Lemma exec_halt_ret_proc `(rec: proc R):
     exec_halt (Ret tt) ---> exec_halt rec.
-  Proof. induction rec; simpl; firstorder. Qed.
+  Proof.
+    rew exec_halt_ret.
+    unfold exec_halt, exec_partial.
+    rew<- bind_star_expand.
+    Left.
+  Qed.
 
   Lemma exec_halt_ret_recover_fold `(rec: proc R):
     _ <- exec_halt (Ret tt); _ <- crash_step; exec_recover rec ---> exec_recover rec.
   Proof.
     setoid_rewrite (exec_halt_ret_proc rec).
     unfold exec_recover.
-    do 2 setoid_rewrite <-bind_assoc.
+    setoid_rewrite <-bind_assoc at 1.
+    setoid_rewrite <-bind_assoc at 1.
     rewrite seq_star_fold; eauto.
   Qed.
+   *)
 
 End Dynamics.
 
